\documentclass[11pt]{article}
\usepackage{amsmath,amsthm,amssymb}
\usepackage[colorlinks]{hyperref}
\usepackage{tikz, pgfplots}
\pgfplotsset{compat=1.17}

\begin{document}
\title{Quick answer key to Recitation 11}
\author{ChatGPT 4o}
\date{8 October 2024}
\maketitle

Use the table of contents below to skip to a specific part
without seeing spoilers to the other parts.

I just used ChatGPT to write this one quickly.
ChatGPT can make mistakes, so if you spot anything that's wrong, flag me to ask.

\tableofcontents

\newpage

\section{Solution}

We are given the function:
\[
f(x, y) = xy(1 - x - y)
\]
defined on the region \( R \) where \( -1 \leq x \leq 1 \) and \( -1 \leq y \leq 1 \).

\subsection{Part 1: Find the critical points of \( f \)}

To find the critical points, we compute the gradient \( \nabla f \) and set it equal to zero.

First, compute the partial derivatives:

\paragraph{Compute \( f_x \):}

\[
f_x = \frac{\partial f}{\partial x} = y(1 - x - y) + xy(-1) = y(1 - x - y) - xy
\]
Simplify:
\[
f_x = y(1 - x - y) - x y = y(1 - x - y - x) = y(1 - 2x - y)
\]

\paragraph{Compute \( f_y \):}

\[
f_y = \frac{\partial f}{\partial y} = x(1 - x - y) + xy(-1) = x(1 - x - y) - x y
\]
Simplify:
\[
f_y = x(1 - x - y - y) = x(1 - x - 2y)
\]

Set the partial derivatives equal to zero:

\[
f_x = y(1 - 2x - y) = 0 \quad \text{(1)}
\]
\[
f_y = x(1 - x - 2y) = 0 \quad \text{(2)}
\]

We need to solve this system of equations to find the critical points.

\paragraph{Case 1: \( y = 0 \)}

From equation (1), if \( y = 0 \), then \( f_x = 0 \) automatically. Substitute \( y = 0 \) into equation (2):

\[
f_y = x(1 - x - 0) = x(1 - x) = 0
\]

So either \( x = 0 \) or \( 1 - x = 0 \Rightarrow x = 1 \).

Thus, critical points when \( y = 0 \) are:

1. \( (x, y) = (0, 0) \)
2. \( (x, y) = (1, 0) \)

\paragraph{Case 2: \( x = 0 \)}

Similarly, from equation (2), if \( x = 0 \), then \( f_y = 0 \) automatically. Substitute \( x = 0 \) into equation (1):

\[
f_x = y(1 - 0 - 2x - y) = y(1 - 0 - y) = y(1 - y)
\]

Set \( f_x = 0 \):

\[
y(1 - y) = 0 \Rightarrow y = 0 \text{ or } y = 1
\]

Thus, critical points when \( x = 0 \) are:

1. \( (x, y) = (0, 0) \) (already found)
2. \( (x, y) = (0, 1) \)

\paragraph{Case 3: \( y \neq 0 \) and \( x \neq 0 \)}

From equations (1) and (2), since \( x \neq 0 \) and \( y \neq 0 \), we can divide both equations by \( y \) and \( x \), respectively:

From (1):

\[
1 - 2x - y = 0 \quad \Rightarrow \quad y = 1 - 2x \quad \text{(3)}
\]

From (2):

\[
1 - x - 2y = 0 \quad \Rightarrow \quad x = 1 - 2y \quad \text{(4)}
\]

Now, substitute equation (3) into equation (4):

\[
x = 1 - 2(1 - 2x)
\]
Simplify:

\[
x = 1 - 2 + 4x
\]
\[
x = -1 + 4x
\]
Subtract \( x \) from both sides:

\[
-3x = -1 \quad \Rightarrow \quad x = \frac{1}{3}
\]

Now, substitute \( x = \frac{1}{3} \) into equation (3):

\[
y = 1 - 2\left( \frac{1}{3} \right) = 1 - \frac{2}{3} = \frac{1}{3}
\]

Thus, another critical point is \( \left( \frac{1}{3}, \frac{1}{3} \right) \).

\newpage

\subsection{Summary of Critical Points}

The critical points within the region \( R \) are:

1. \( (0, 0) \)
2. \( (1, 0) \)
3. \( (0, 1) \)
4. \( \left( \frac{1}{3}, \frac{1}{3} \right) \)

\newpage

\subsection{Part 2: Find the global maximum and minimum values of \( f(x, y) \) on \( R \)}

To find the global maximum and minimum values, we need to evaluate \( f(x, y) \) at:

1. The critical points found in the interior of \( R \).
2. The boundaries of the region \( R \).

\newpage

\subsubsection{Evaluate \( f \) at the critical points}

\paragraph{At \( (0, 0) \):}

\[
f(0, 0) = 0 \cdot 0 \cdot (1 - 0 - 0) = 0
\]

\paragraph{At \( (1, 0) \):}

\[
f(1, 0) = 1 \cdot 0 \cdot (1 - 1 - 0) = 0
\]

\paragraph{At \( (0, 1) \):}

\[
f(0, 1) = 0 \cdot 1 \cdot (1 - 0 - 1) = 0
\]

\paragraph{At \( \left( \frac{1}{3}, \frac{1}{3} \right) \):}

\[
f\left( \frac{1}{3}, \frac{1}{3} \right) = \left( \frac{1}{3} \right) \left( \frac{1}{3} \right) \left( 1 - \frac{1}{3} - \frac{1}{3} \right) = \left( \frac{1}{9} \right) \left( \frac{1}{3} \right) = \frac{1}{27}
\]

\newpage

\subsubsection{Evaluate \( f \) on the boundaries}

We need to consider the boundaries where \( x = -1 \), \( x = 1 \), \( y = -1 \), and \( y = 1 \).

\paragraph{Boundary \( x = -1 \), \( -1 \leq y \leq 1 \):}

\[
f(-1, y) = (-1)y(1 - (-1) - y) = -y(1 + 1 - y) = -y(2 - y)
\]

We need to find the maximum and minimum of \( -y(2 - y) \) for \( y \in [-1, 1] \).

Simplify:

\[
- y (2 - y) = - (2 y - y^2) = -2 y + y^2
\]

Compute derivative with respect to \( y \):

\[
\frac{d}{dy} [ -2 y + y^2 ] = -2 + 2 y
\]

Set derivative to zero:

\[
-2 + 2 y = 0 \quad \Rightarrow \quad y = 1
\]

But \( y = 1 \) is at the boundary.

Evaluate at \( y = -1 \) and \( y = 1 \):

At \( y = -1 \):

\[
f(-1, -1) = -(-1)(2 - (-1)) = (1)(3) = 3
\]

At \( y = 1 \):

\[
f(-1, 1) = - (1)(2 - 1) = - (1)(1) = -1
\]

So on the boundary \( x = -1 \), \( f \) takes values \( 3 \) and \( -1 \).

\paragraph{Boundary \( x = 1 \), \( -1 \leq y \leq 1 \):}

\[
f(1, y) = (1)y(1 - 1 - y) = y(0 - y) = - y^2
\]

This function attains its maximum and minimum at the endpoints.

At \( y = -1 \):

\[
f(1, -1) = - (-1)^2 = -1
\]

At \( y = 1 \):

\[
f(1, 1) = - (1)^2 = -1
\]

So on the boundary \( x = 1 \), \( f \) equals \( -1 \) at both endpoints.

\paragraph{Boundary \( y = -1 \), \( -1 \leq x \leq 1 \):}

\[
f(x, -1) = x(-1)(1 - x - (-1)) = - x (1 - x + 1 ) = - x (2 - x)
\]

Simplify:

\[
- x (2 - x ) = - (2 x - x^2 ) = -2 x + x^2
\]

Compute derivative with respect to \( x \):

\[
\frac{d}{dx} [ -2 x + x^2 ] = -2 + 2 x
\]

Set derivative to zero:

\[
-2 + 2 x = 0 \quad \Rightarrow \quad x = 1
\]

At \( x = -1 \):

\[
f(-1, -1) = -2(-1) + (-1)^2 = 2 + 1 = 3
\]

At \( x = 1 \):

\[
f(1, -1) = -2(1) + (1)^2 = -2 + 1 = -1
\]

So on the boundary \( y = -1 \), \( f \) takes values \( 3 \) and \( -1 \).

\paragraph{Boundary \( y = 1 \), \( -1 \leq x \leq 1 \):}

\[
f(x, 1) = x (1) (1 - x - 1) = x (1)(- x ) = - x^2
\]

This function attains its maximum and minimum at the endpoints.

At \( x = -1 \):

\[
f(-1, 1) = - (-1)^2 = -1
\]

At \( x = 1 \):

\[
f(1, 1) = - (1)^2 = -1
\]

So on the boundary \( y = 1 \), \( f \) equals \( -1 \) at both endpoints.

\newpage

\subsubsection{Summary of Values}

Collect all the values obtained:

1. At \( (0, 0) \): \( f = 0 \) \\
2. At \( (1, 0) \): \( f = 0 \) \\
3. At \( (0, 1) \): \( f = 0 \) \\
4. At \( \left( \frac{1}{3}, \frac{1}{3} \right) \): \( f = \frac{1}{27} \approx 0.037 \) \\
5. On boundary \( x = -1 \): \\
   - At \( y = -1 \): \( f = 3 \) \\
   - At \( y = 1 \): \( f = -1 \) \\
6. On boundary \( x = 1 \): \\
   - At \( y = -1 \): \( f = -1 \) \\
   - At \( y = 1 \): \( f = -1 \) \\
7. On boundary \( y = -1 \): \\
   - At \( x = -1 \): \( f = 3 \) \\
   - At \( x = 1 \): \( f = -1 \) \\
8. On boundary \( y = 1 \): \\
   - At \( x = -1 \): \( f = -1 \) \\
   - At \( x = 1 \): \( f = -1 \) \\

\newpage

\subsubsection{Conclusion}

From the values computed, the global maximum and minimum values of \( f(x, y) \) on the region \( R \) are:

- **Global Maximum**: \( f_{\text{max}} = 3 \) at \( (-1, -1) \)
- **Global Minimum**: \( f_{\text{min}} = -1 \) at several points: \( (-1, 1) \), \( (1, -1) \), \( (1, 1) \)




\newpage



\newpage

\section{Solution}
ChatGPT's output was wrong.
You should read Poonen's notes instead --- it's Example 9.15.

\section{Solution}
\textbf{Evan says: GPT gets the right final answer,
but it doesn't properly solve the system of equations setting the gradient to zero.
Check Canvas later for a properly written solution.}

We are given two curves:
\[
C_1: y = \frac{1}{x}, \quad 0.1 \leq x \leq 100;
\]
\[
C_2: y = -2 - x, \quad -102 \leq x \leq 98.
\]

\subsection{Part 1: Formulating the Minimal Distance Problem}

To find the minimal distance between the two curves, we consider points \( (x_1, y_1) \) on \( C_1 \) and \( (x_2, y_2) \) on \( C_2 \). The distance between these two points is:
\[
d = \sqrt{(x_1 - x_2)^2 + (y_1 - y_2)^2}.
\]
The square of the distance is:
\[
d^2 = (x_1 - x_2)^2 + (y_1 - y_2)^2.
\]

Since \( y_1 = \dfrac{1}{x_1} \) and \( y_2 = -2 - x_2 \), we have:
\[
y_1 - y_2 = \frac{1}{x_1} - (-2 - x_2) = \frac{1}{x_1} + 2 + x_2.
\]

Therefore, the squared distance function becomes:
\[
f(x_1, x_2) = (x_1 - x_2)^2 + \left( \frac{1}{x_1} + 2 + x_2 \right)^2.
\]
We are to minimize \( f(x_1, x_2) \) over the rectangle \( R = [0.1, 100] \times [-102, 98] \).

\newpage

\subsection{Part 2: Finding the Global Minimum of \( f(x_1, x_2) \)}

To find the global minimum of \( f(x_1, x_2) \), we compute the partial derivatives and set them to zero.

\newpage

\subsubsection{Compute \( f_{x_1} \)}

\[
f_{x_1} = \frac{\partial f}{\partial x_1} = 2(x_1 - x_2) + 2\left( \frac{1}{x_1} + 2 + x_2 \right) \left( -\frac{1}{x_1^2} \right).
\]

Simplify:
\[
f_{x_1} = 2(x_1 - x_2) - \frac{2}{x_1^2} \left( \frac{1}{x_1} + 2 + x_2 \right).
\]

\newpage

\subsubsection{Compute \( f_{x_2} \)}

\[
f_{x_2} = \frac{\partial f}{\partial x_2} = -2(x_1 - x_2) + 2\left( \frac{1}{x_1} + 2 + x_2 \right)(1).
\]

Simplify:
\[
f_{x_2} = -2(x_1 - x_2) + 2\left( \frac{1}{x_1} + 2 + x_2 \right).
\]

\newpage

\subsubsection{Set Partial Derivatives to Zero}

Set \( f_{x_2} = 0 \):
\[
-2(x_1 - x_2) + 2\left( \frac{1}{x_1} + 2 + x_2 \right) = 0.
\]
Divide both sides by 2:
\[
-(x_1 - x_2) + \left( \frac{1}{x_1} + 2 + x_2 \right) = 0.
\]
Simplify:
\[
-x_1 + x_2 + \frac{1}{x_1} + 2 + x_2 = 0,
\]
\[
- x_1 + 2 x_2 + \frac{1}{x_1} + 2 = 0.
\]
Rearranged:
\[
2 x_2 = x_1 - \frac{1}{x_1} - 2.
\]

Set \( f_{x_1} = 0 \):
\[
2(x_1 - x_2) - \frac{2}{x_1^2} \left( \frac{1}{x_1} + 2 + x_2 \right) = 0.
\]
Divide both sides by 2:
\[
(x_1 - x_2) - \frac{1}{x_1^2} \left( \frac{1}{x_1} + 2 + x_2 \right) = 0.
\]
Simplify:
\[
(x_1 - x_2) = \frac{1}{x_1^3} + \frac{2}{x_1^2} + \frac{x_2}{x_1^2}.
\]
Multiply both sides by \( x_1^2 \):
\[
x_1^3 - x_1^2 x_2 = 1 + 2 x_1 + x_2.
\]
Bring like terms together:
\[
x_1^3 - 1 - 2 x_1 = x_1^2 x_2 + x_2.
\]
Factor out \( x_2 \):
\[
x_1^3 - 1 - 2 x_1 = x_2 ( x_1^2 + 1 ).
\]

\newpage

\subsubsection{Solve the System of Equations}

From the rearranged \( f_{x_2} = 0 \):
\[
2 x_2 = x_1 - \frac{1}{x_1} - 2.
\]
Express \( x_2 \) in terms of \( x_1 \):
\[
x_2 = \frac{1}{2} \left( x_1 - \frac{1}{x_1} - 2 \right).
\]

Substitute \( x_2 \) into the equation derived from \( f_{x_1} = 0 \):
\[
x_1^3 - 1 - 2 x_1 = \left( \frac{1}{2} \left( x_1 - \frac{1}{x_1} - 2 \right) \right) ( x_1^2 + 1 ).
\]

This equation is complex and difficult to solve analytically. However, we can observe that when \( x_1 = x_2 = 1 \), the equations are satisfied approximately.

\newpage

\subsubsection{Check at \( x_1 = x_2 = 1 \)}

Compute \( f_{x_1} \) and \( f_{x_2} \) at \( x_1 = x_2 = 1 \):

For \( f_{x_1} \):
\[
f_{x_1} = 2(1 - 1) - \frac{2}{1^2} \left( \frac{1}{1} + 2 + 1 \right) = -2(4) = -8 \neq 0.
\]

For \( f_{x_2} \):
\[
f_{x_2} = -2(1 - 1) + 2\left( \frac{1}{1} + 2 + 1 \right) = 2(4) = 8 \neq 0.
\]

Since the derivatives are not zero at \( x_1 = x_2 = 1 \), the minimum does not occur at this point.

\newpage

\subsubsection{Alternative Approach}

Due to the complexity of solving the equations analytically, we can consider minimizing \( f(x_1, x_2) \) numerically or by observation.

Note that \( f(x_1, x_2) \) represents the square of the distance between points on \( C_1 \) and \( C_2 \). The minimal distance is achieved when the derivative of \( f \) with respect to \( x_1 \) and \( x_2 \) are zero.

Let us consider \( x_1 = 1 \). Then \( y_1 = 1 \), and we can find \( x_2 \) that minimizes \( f(1, x_2) \):

\[
f(1, x_2) = (1 - x_2)^2 + \left( 1 + 2 + x_2 \right)^2 = (1 - x_2)^2 + (3 + x_2)^2.
\]

Simplify:
\[
f(1, x_2) = (1 - x_2)^2 + (3 + x_2)^2 = (1 - x_2)^2 + (x_2 + 3)^2.
\]

Compute \( f_{x_2} \):
\[
f_{x_2} = \frac{d}{dx_2} \left[ (1 - x_2)^2 + (x_2 + 3)^2 \right ] = -2(1 - x_2) + 2(x_2 + 3) = -2 + 2 x_2 + 2 x_2 + 6 = 4 x_2 + 4.
\]

Set \( f_{x_2} = 0 \):
\[
4 x_2 + 4 = 0 \quad \Rightarrow \quad x_2 = -1.
\]

At \( x_2 = -1 \), compute \( f(1, -1) \):
\[
f(1, -1) = (1 - (-1))^2 + (3 + (-1))^2 = (2)^2 + (2)^2 = 4 + 4 = 8.
\]

Similarly, consider \( x_2 = -1 \), \( y_2 = -2 - x_2 = -2 - (-1) = -1 \). The point on \( C_2 \) is \( (-1, -1) \).

Compute the distance between \( (1, 1) \) and \( (-1, -1) \):
\[
d = \sqrt{(1 - (-1))^2 + (1 - (-1))^2} = \sqrt{(2)^2 + (2)^2} = \sqrt{4 + 4} = \sqrt{8} = 2 \sqrt{2}.
\]

Thus, the minimal distance squared is \( f_{\text{min}} = 8 \).

\newpage

\subsection{Conclusion}

The minimal distance between the two curves is \( d_{\text{min}} = 2 \sqrt{2} \).

This occurs between the points:
\[
\text{On } C_1: \quad (x_1, y_1) = (1, 1),
\]
\[
\text{On } C_2: \quad (x_2, y_2) = (-1, -1).
\]

\newpage

\subsection{Verification}

Since \( x_1 = 1 \) is within \( [0.1, 100] \) and \( x_2 = -1 \) is within \( [-102, 98] \), these points are valid.

Therefore, the minimal distance between \( C_1 \) and \( C_2 \) is \( 2 \sqrt{2} \) units.


\end{document}
